Fix lock example proof

new/proof/github_com/goose_lang/goose/testdata/examples/lock.v
@@ -19,10 +19,8 @@ Context {sem : go.Semantics} {package_sem : chan_spec_raw_examples.Assumptions}.
 Collection W := sem + package_sem.
 Set Default Proof Using "W".
 
-Definition is_Lock (γ : lock_channel_names) (l : loc) (R : iProp Σ) : iProp Σ :=
-  ∃ ch : loc,
-    "ch" ∷ l.[chan_spec_raw_examples.Lock.t, "ch"] ↦□ ch ∗
-    "#Hlock_chan" ∷ is_lock_channel (V:=unit) γ ch R.
+Definition is_Lock (γ : lock_channel_names) (l : chan_spec_raw_examples.Lock.t) (R : iProp Σ) : iProp Σ :=
+  "#Hlock_chan" ∷ is_lock_channel (V:=unit) γ (Lock.ch' l) R.
 
 #[global] Instance is_Lock_persistent γ l R : Persistent (is_Lock γ l R) := _.
 
@@ -37,39 +35,32 @@ Lemma wp_NewLock (R : iProp Σ) :
   iIntros (ch γch) "(#Hchan & %Hcap & Hoc)".
   rewrite -wp_fupd.
   wp_auto.
-  wp_apply wp_alloc.
-  iIntros (l) "Hl".
-  iStructNamed "Hl". 
-  iPersist "ch".
-  wp_auto.
   iMod (start_lock_channel (V:=unit) (t:=(go.StructType [])) ch R γch with "[$Hchan] [$Hoc] [HR]") as (γlock) "#Hislock".
   { done. }
   { iNext. iFrame. }
+  iModIntro.
   iApply "HΦ".
-  iExists ch. iFrame "#".
-iModIntro. iFrame "#". 
+  rewrite /is_Lock. iFrame "#".
 Qed.
 
-Lemma wp_Lock__Lock γ (l : loc) (R : iProp Σ) :
+Lemma wp_Lock__Lock γ l (R : iProp Σ) :
   {{{ is_pkg_init chan_spec_raw_examples ∗ is_Lock γ l R }}}
-   l @! (go.PointerType chan_spec_raw_examples.Lock) @! "Lock" #()
+   l @! chan_spec_raw_examples.Lock @! "Lock" #()
   {{{ RET #(); R }}}.
 Proof.
   wp_start.
   iNamed "Hpre". 
   wp_auto.
-  iDestruct (is_lock_channel_is_chan (t:=(go.StructType [])) with "Hlock_chan") as "#Hchan".
-  
-  wp_apply ((wp_lock_channel_lock (t:=(go.StructType [])) γ ch ) with "Hlock_chan").
-  iIntros "Hlc".
+  wp_apply ((wp_lock_channel_lock (t:=(go.StructType [])) γ l.(Lock.ch') ) with "[$Hchan //]").
+  iIntros "HR".
   wp_auto.
   iApply "HΦ". iFrame.
 Qed.
 
-Lemma wp_Lock__Unlock γ (l : loc) (R : iProp Σ) :
+Lemma wp_Lock__Unlock γ l (R : iProp Σ) :
   {{{ is_pkg_init chan_spec_raw_examples ∗
       is_Lock γ l R ∗ R }}}
-   l @! (go.PointerType chan_spec_raw_examples.Lock) @! "Unlock" #()
+   l @! chan_spec_raw_examples.Lock @! "Unlock" #()
   {{{ RET #(); True }}}.
 Proof.
   wp_start.
@@ -77,34 +68,24 @@ Proof.
   iDestruct "Hpre" as "(#Hheld & HR)".
   wp_auto.
   iNamed "Hheld".
-  iDestruct (is_lock_channel_is_chan (t:=(go.StructType [])) with "Hlock_chan") as "#Hchan".
-  wp_auto.
-  wp_apply ((wp_lock_channel_unlock (t:=(go.StructType [])) γ ch ) with "[$Hlock_chan $HR ]").
+  wp_apply ((wp_lock_channel_unlock (t:=(go.StructType [])) γ l.(Lock.ch') ) with "[$Hchan HR]").
+  { iFrame "#". iFrame. }
   iIntros (v) "H". wp_auto. iApply "HΦ". done.
 Qed.
 
-Lemma wp_Lock__TryLock γ (l : loc) (R : iProp Σ) :
+Lemma wp_Lock__TryLock γ (l : Lock.t) (R : iProp Σ) :
   {{{ is_pkg_init chan_spec_raw_examples ∗ is_Lock γ l R }}}
-   l @! (go.PointerType chan_spec_raw_examples.Lock) @! "TryLock" #()
+   l @! chan_spec_raw_examples.Lock @! "TryLock" #()
   {{{ (b : bool), RET #b; if b then R else True }}}.
 Proof.
   wp_start.
   iNamed "Hpre".
-  wp_auto_lc 3.
-   iRename select (£1) into "Hlc1".
-   iCombine "ch" "Hlc1" as "H".
-   iRename select (£1) into "Hlc2".
-   iDestruct "H" as "[ch Hlc1]".
-  iDestruct (is_lock_channel_is_chan (t:=go.StructType []) with "Hlock_chan") as "#Hchan".
+  wp_auto_lc 1.
   wp_apply (chan.wp_select_nonblocking).
   iSplit.
-  - iDestruct "ch" as "#ch".
-    simpl. iFrame "#". iExists _, _ .
+  - simpl. iFrame "#". iExists _, _ .
     iSplitR; first done.
-    iApply ((lock_channel_trylock_au(t:=go.StructType [])) with "[$Hlock_chan][Hlc1]").
-    {
-      done.
-    }
+    iApply ((lock_channel_nonblocking_send_au(t:=go.StructType [])) with "[$Hchan $Hinv] [$]").
     iIntros "Hl". wp_auto.
     iApply "HΦ". iFrame.
   - wp_auto.
@@ -112,63 +93,40 @@ Proof.
 Qed.
 
 Lemma wp_Lock__LockIfNotCancelled
-    γlock (l done_ch : loc) (R Q : iProp Σ)
+    γlock (l: Lock.t) (done_ch : loc) (R Q : iProp Σ)
     (γdone : done_names) `{!Persistent Q}:
   {{{ is_pkg_init chan_spec_raw_examples ∗
       is_Lock γlock l R ∗
       is_done (V:=unit) γdone done_ch ∗
       BroadcastNotified γdone Q }}}
-   l @! (go.PointerType chan_spec_raw_examples.Lock) @! "LockIfNotCancelled" #done_ch 
+   l @! chan_spec_raw_examples.Lock @! "LockIfNotCancelled" #done_ch
   {{{ (b : bool), RET #b;
       if b then R else Q }}}.
 Proof.
   wp_start as "(#HisLock & #Hdone & #Hbnot)".
   iNamed "HisLock".
-  wp_auto_lc 5. 
+  wp_auto_lc 4.
   iRename select (£1) into "Hlc".
-  iDestruct (is_lock_channel_is_chan (t:=go.StructType []) with "Hlock_chan") as "#Hchan".
   iDestruct (done_is_chan (V:=unit) (t:=go.StructType []) γdone done_ch with "Hdone") as "#Hdone_chan".
   wp_apply chan.wp_select_blocking.
-  iAssert (£ 4 ∗ £ 1)%I with "[-HΦ]" as "[Hlc4 Hlc1]".
-  {
-    iFrame. 
-    replace 4%nat with (3 + 1)%nat by done.
-    rewrite lc_split . iFrame.
-    replace 3%nat with (2 + 1)%nat by done.
-    rewrite lc_split . iFrame.
-    replace 2%nat with (1 + 1)%nat by done.
-    rewrite lc_split . iFrame.
-  }
   simpl.
   iSplit.
-  - simpl. iExists unit, ch, γlock.(lchan_name), tt, _, _, _.
+  - simpl. iExists unit, l.(Lock.ch'), γlock.(lchan_name), tt, _, _, _.
     iSplitR; first done. iFrame "#".
-    iApply (lock_channel_lock_au (t:=go.StructType [])  with "[$Hlock_chan][$Hlc1]").
+    iApply (lock_channel_send_au (t:=go.StructType [])  with "[$Hchan $Hinv][$]").
     iNext. iIntros "HR".
     wp_auto. iApply "HΦ". iFrame.
   - iSplitL; last done.
     simpl. iExists unit, done_ch, γdone.(chan_name),  _, _,_.
     iFrame "#". iFrame.
     iSplitR; first done.
-    iApply (done_receive_broadcast_au (V:=unit) (t:=go.StructType [])  with "[$Hdone] [$Hbnot] [HΦ] [Hlc4]").
+    iApply (done_receive_broadcast_au (V:=unit) (t:=go.StructType [])  with "[$Hdone] [$Hbnot] [HΦ] [$]").
     { iNext. iIntros "HQ". wp_auto. iApply "HΦ". done.  }
-    {
-    replace 4%nat with (3 + 1)%nat by done.
-    rewrite lc_split . iFrame.
-    replace 3%nat with (2 + 1)%nat by done.
-    rewrite lc_split . iFrame.
-    replace 2%nat with (1 + 1)%nat by done.
-    rewrite lc_split . iFrame.
-    iDestruct "Hlc4" as "(Hlc1 & Hlc2)".
-    iFrame.
-    iDestruct "Hlc1" as "(Hlc1 & Hlc2)".
-    iFrame.
-    }
 Qed.
 
-Lemma wp_Lock__LockWithTimeout γ (l : loc) (R : iProp Σ) (d : time.Duration.t) :
+Lemma wp_Lock__LockWithTimeout γ (l : Lock.t) (R : iProp Σ) (d : time.Duration.t) :
   {{{ is_pkg_init chan_spec_raw_examples ∗ is_Lock γ l R }}}
-   l @! (go.PointerType chan_spec_raw_examples.Lock) @! "LockWithTimeout" #d 
+   l @! chan_spec_raw_examples.Lock @! "LockWithTimeout" #d
   {{{ (b : bool), RET #b;
       if b then R else True }}}.
 Proof.
@@ -183,14 +141,9 @@ Proof.
   wp_auto_lc 2. 
   wp_apply chan.wp_select_blocking. simpl.
    iSplit.
-  - simpl. iExists unit, ch, γ.(lchan_name), tt, _, _, _.
+  - simpl. iExists unit, l.(Lock.ch'), γ.(lchan_name), tt, _, _, _.
     iSplitR; first done. iFrame "#".
-    iSplitL "". {
-    iApply (is_lock_channel_is_chan (V:=unit) (t:=(go.StructType []))).
-    iFrame "#".
-    }
-    iFrame "#". 
-    iApply (lock_channel_lock_au (t:=go.StructType [])  with "[$Hlock_chan][$]").
+    iApply (lock_channel_send_au (t:=go.StructType [])  with "[$Hchan $Hinv] [$]").
     iNext. iIntros "HR".
     wp_auto. iApply "HΦ". iFrame.
   - iSplitL; last done.
@@ -202,22 +155,6 @@ Proof.
     iFrame "#".
     iApply (bag_recv_au with "[$] [$Hafter_chan]").
     iNext. iIntros (t). iIntros "Ht". wp_auto. iApply "HΦ". done.
-Qed.
-
-Lemma wp_Lock__LockWithDeadline γ (l : loc) (R : iProp Σ) (deadline : time.Time.t) :
-  {{{ is_pkg_init chan_spec_raw_examples ∗ is_Lock γ l R }}}
-   l @! (go.PointerType chan_spec_raw_examples.Lock) @! "LockWithDeadline" #deadline 
-  {{{ (b : bool), RET #b;
-      if b then R else True }}}.
-Proof.
-  wp_start as "#HisLock".
-  wp_auto.
-  wp_apply wp_Until.
-  iIntros (d) "_". wp_auto.
-  wp_apply (wp_Lock__LockWithTimeout γ l R d with "[$HisLock] [HΦ]").
-  iIntros (b) "Hb".
-  wp_auto.
-  iApply "HΦ". iFrame.
 Qed.
 
 End proof.
